wip lemmas

Untangle.v
@@ -1,12 +1,628 @@
-Require Export SystemFR.ReducibilityLemmas.
+Require Export SystemFR.ScalaDepSugar.
+Require Export SystemFR.ReducibilitySubtype.
+Require Export SystemFR.EquivalentContext.
+Require Export SystemFR.TOpenTClose.
+Require Export SystemFR.CloseLemmas.
 
-Inductive untangle: tree -> tree -> Prop :=
-| UntangleRefl: forall T, untangle T T
+Opaque reducible_values.
+
+Parameter T_key: tree.
+Parameter T_map: tree.
+Hypothesis key_fv: forall tag, pfv T_key tag = nil.
+Hypothesis map_fv: forall tag, pfv T_map tag = nil.
+Hypothesis key_wf: forall k, wf T_key k.
+Hypothesis map_wf: forall k, wf T_map k.
+
+Definition T_trail: tree := T_prod T_key T_map.
+
+Lemma substitute_map:
+  forall l tag, psubstitute T_map l tag = T_map.
+Proof.
+  intros; apply substitute_nothing5; eauto using map_fv.
+Qed.
+
+Lemma substitute_key:
+  forall l tag, psubstitute T_key l tag = T_key.
+Proof.
+  intros; apply substitute_nothing5; eauto using key_fv.
+Qed.
+
+Lemma substitute_trail:
+  forall l tag, psubstitute T_trail l tag = T_trail.
+Proof.
+  repeat step || rewrite substitute_map || rewrite substitute_key.
+Qed.
+
+Opaque T_trail.
+
+Definition app2 f a b := app (app f a) b.
+Definition app3 f a b c := app (app (app f a) b) c.
+
+(* tlookup: T_map -> T_key -> T_top *)
+Parameter tlookup: tree -> tree -> tree.
+
+(* concat: T_key -> T_key -> T_key *)
+Parameter concat: tree -> tree -> tree.
+
+(* prefix: T_key -> T_key -> T_bool *)
+Parameter prefix: tree -> tree -> tree.
+
+Parameter empty_map: tree (* T_map *).
+Hypothesis empty_map_type: [ empty_map : T_map ].
+
+(* update: T_key -> T_key -> T_map -> T_map -> T_map *)
+Parameter update: tree -> tree -> tree -> tree -> tree.
+
+(* `update` returns a map such that the submap rooted at `old_key` is now rooted at `new_key` *)
+(*  forall key fresh_key fresh_map map δ,
+    [ tlookup fresh_map (concat fresh_key δ) ≡
+      tlookup (update key fresh_key fresh_map map) (concat key δ) ] *)
+
+(* `update`'s are commutative when keys are not prefixes of one another *)
+Hypothesis update_spec:
+  forall key1 fresh_key1 fresh_map1 key2 fresh_key2 fresh_map2 map,
+    [ key1 : T_key ] ->
+    [ key2 : T_key ] ->
+    [ fresh_key1 : T_key ] ->
+    [ fresh_key2 : T_key ] ->
+    [ fresh_map1 : T_map ] ->
+    [ fresh_map2 : T_map ] ->
+    [ map : T_map ] ->
+    [ prefix fresh_key1 fresh_key2 ≡ tfalse ] ->
+    [ prefix fresh_key2 fresh_key1 ≡ tfalse ] ->
+    [ update key1 fresh_key1 fresh_map1 (update key2 fresh_key2 fresh_map2 map) ≡
+      update key2 fresh_key2 fresh_map2 (update key1 fresh_key1 fresh_map1 map) ].
+
+(*
+Hypothesis update_spec3:
+  forall key fresh_key fresh_map map key',
+    [ prefix key key' ≡ tfalse ] ->
+    [ tlookup map key' ≡ tlookup (update key fresh_key fresh_map map) key' ].
+*)
+
+(* Terms that take a map and a key `k`, and only lookup the map on keys greater or
+   equal than `k` satisfy the following property, described by the type `T_tau` *)
+Parameter T_tau: tree.
+Lemma tau_property:
+  forall f key fresh_key fresh_map map,
+    [ f : T_tau ] ->
+    [ app2 f fresh_map fresh_key ≡ app2 f (update key fresh_key fresh_map map) key ].
+Admitted.
+
+Ltac equivalent_refl :=
+  match goal with
+  | |- [ _ ≡ _ ] => apply equivalent_refl
+  end.
+
+Lemma tau2_example:
+  forall f1 f2 fresh_key1 fresh_key2 fresh_map1 fresh_map2 key1 key2,
+    [ f1 : T_tau ] ->
+    [ f2 : T_tau ] ->
+    [ key1 : T_key ] ->
+    [ key2 : T_key ] ->
+    [ fresh_key1 : T_key ] ->
+    [ fresh_key2 : T_key ] ->
+    [ fresh_map1 : T_map ] ->
+    [ fresh_map2 : T_map ] ->
+    [ prefix fresh_key1 fresh_key2 ≡ tfalse ] ->
+    [ prefix fresh_key2 fresh_key1 ≡ tfalse ] ->
+    exists map,
+      [ app2 f1 fresh_map1 fresh_key1 ≡ app2 f1 map key1 ] /\
+      [ app2 f2 fresh_map2 fresh_key2 ≡ app2 f2 map key2 ].
+Proof.
+  intros.
+  exists (update key1 fresh_key1 fresh_map1 (update key2 fresh_key2 fresh_map2 empty_map)); steps.
+  - pose proof (tau_property _ key1 fresh_key1 fresh_map1
+      (update key2 fresh_key2 fresh_map2 empty_map) H); auto.
+  - pose proof (tau_property _ key2 fresh_key2 fresh_map2
+      (update key1 fresh_key1 fresh_map1 empty_map) H0); auto.
+    eapply equivalent_trans; eauto;
+      repeat apply equivalent_app || apply update_spec || equivalent_refl;
+      eauto 2 using reducible_erased with step_tactic;
+      eauto 2 using reducible_wf with step_tactic;
+      eauto 2 using reducible_fv with step_tactic;
+      eauto using empty_map_type.
+Qed.
+
+Fixpoint closes k T xs :=
+  match xs with
+  | nil => T
+  | x :: xs => close k (closes (S k) T xs) x
+  end.
+
+Fixpoint T_existss n T1 T2 :=
+  match n with
+  | 0 => T2
+  | S n' => T_exists T1 (T_existss n' T1 T2)
+  end.
+
+Definition T_exists_vars xs T1 T2 :=
+  T_existss (List.length xs) T1 (closes 0 T2 xs).
+
+Definition incomparable (keys : list tree) : Prop.
+Admitted.
+
+(* Using the tau property, we can untangle *)
+Inductive untangle: context -> tree -> tree -> Prop :=
+| UntangleFreshen:
+    forall Γ f T T' template xs ys keys m,
+      List.NoDup (xs ++ ys) ->
+      T  = substitute template
+        (List.combine xs (List.map (fun key => app f (pp key (fvar m term_var))) keys)) ->
+      T' = substitute template
+        (List.combine xs (List.map (fun y => app f (fvar y term_var)) ys)) ->
+      untangle Γ
+               (T_exists T_trail (close 0 T m))
+               (T_exists_vars ys T_trail T')
+
+| UntangleRefl: forall Γ T, untangle Γ T T
 .
 
-Lemma untangle_open_equivalent_types:
-  forall Θ Γ T1 T2,
-    untangle T1 T2 ->
-    [ Θ; Γ ⊨ T1 = T2 ].
+Opaque List.
+
+Lemma wfs_combine:
+  forall l1 l2 k T,
+    List.Forall (fun t => [ t : T ]) l2 ->
+    wfs (List.combine l1 l2) k.
 Proof.
+  induction l1; steps; eauto 3 with wf step_tactic.
+Qed.
+
+Lemma wf_var:
+  forall n k, wf (fvar n term_var) k.
+Proof. steps. Qed.
+
+Lemma wfs_combine2:
+  forall xs f keys m,
+    wf f 0 ->
+    List.Forall (fun key => [ key : T_key ]) keys ->
+    wfs (List.combine xs (List.map (fun key : tree => app f (pp key (fvar m term_var))) keys)) 0.
+Proof.
+  induction xs; destruct keys; steps; eauto with wf.
+Qed.
+
+Lemma lookup_combine_map:
+  forall eq_dec (xs: list nat) f l (t1 t2: tree) x,
+    lookup eq_dec (List.combine xs l) x = Some t1 ->
+    lookup eq_dec (List.combine xs (List.map f l)) x = Some t2 ->
+    t2 = f t1.
+Proof.
+  induction xs; repeat step; eauto.
+Qed.
+
+Lemma lookup_combine_some_none:
+  forall eq_dec (xs: list nat) (l1 l2: list tree) t x,
+    List.length l1 = List.length l2 ->
+    lookup eq_dec (List.combine xs l1) x = Some t ->
+    lookup eq_dec (List.combine xs l2) x = None ->
+    False.
+Proof.
+  induction xs; steps; eauto.
+Qed.
+
+Lemma psubstitute_texistss:
+  forall n T1 T2 l tag,
+    psubstitute (T_existss n T1 T2) l tag =
+    T_existss n (psubstitute T1 l tag) (psubstitute T2 l tag).
+Proof.
+  induction n; steps.
+Qed.
+
+Lemma substitute_closes:
+  forall xs t l tag k,
+    (forall x, x ∈ support l -> x ∈ xs -> False) ->
+    pclosed_mapping l term_var ->
+    psubstitute (closes k t xs) l tag = closes k (psubstitute t l tag) xs.
+Proof.
+  induction xs;
+    repeat step || rewrite substitute_close by (steps; eauto);
+    try solve [ rewrite_any; steps; eauto ].
+Qed.
+
+Lemma psubstitute_texists_vars:
+  forall xs T1 T2 l tag,
+    (forall x, x ∈ support l -> x ∈ xs -> False) ->
+    pclosed_mapping l term_var ->
+    psubstitute (T_exists_vars xs T1 T2) l tag =
+    T_exists_vars xs (psubstitute T1 l tag) (psubstitute T2 l tag).
+Proof.
+  unfold T_exists_vars; intros; rewrite psubstitute_texistss; apply f_equal.
+  rewrite substitute_closes; steps; eauto.
+Qed.
+
+Lemma subst_subst:
+  forall t l ts xs tag,
+    (forall x, x ∈ pfv t tag -> x ∈ support l -> False) ->
+    psubstitute (psubstitute t (List.combine xs ts) tag) l tag =
+    psubstitute t (List.combine xs (List.map (fun t' => psubstitute t' l tag) ts)) tag.
+Proof.
+  induction t; repeat step || t_equality;
+    eauto 4 using lookup_combine_some_none, List.map_length with exfalso;
+    try solve [ rewrite_any; steps; eapply_any; repeat step || list_utils; eauto ];
+    try solve [ eapply_anywhere lookup_combine_map; eauto ];
+    try solve [ t_lookup; eauto with exfalso ].
+Qed.
+
+Lemma list_map_subst:
+  forall l f t m v,
+    (forall e, e ∈ l -> m ∈ fv e -> False) ->
+    List.map (fun e => app f (pp (psubstitute e ((m, v) :: nil) term_var) t)) l =
+    List.map (fun e => app f (pp e t)) l.
+Proof.
+  induction l; repeat step || t_substitutions || t_equality; eauto.
+Qed.
+
+Fixpoint opens k t reps :=
+  match goal with
+  | 
+
+Lemma reducible_existss:
+  forall xs ρ v vs T1 T2,
+    List.Forall (fun v => [ ρ | v : T1 ]v) vs =
+    [ ρ | v : opens 0 T2 vs ]v ->
+    [ ρ | v : T_existss n T1 T2 ]v.
+Proof.
+  unfold T_exists_vars; steps.
 Admitted.
+
+Lemma reducible_exists_vars:
+  forall xs ρ v vs T1 T2,
+    List.Forall (fun v => [ ρ | v : T1 ]v) vs =
+    [ ρ | v : psubstitute T2 (List.combine xs vs) term_var ]v ->
+    [ ρ | v : T_exists_vars xs T1 T2 ]v.
+Proof.
+  unfold T_exists_vars; steps.
+Admitted.
+
+Lemma untangle_freshen:
+forall Γ f template xs ys keys m,
+  List.NoDup (xs ++ ys) ->
+  wf template 0 ->
+  wf f 0 ->
+  List.Forall (fun key => [ key : T_key ]) keys ->
+  ~ m ∈ fv template ->
+  ~ m ∈ fv f ->
+  (forall key, key ∈ keys -> m ∈ fv key -> False) ->
+  (forall y, y ∈ ys -> y ∈ support Γ -> False) ->
+  [Γ
+  ⊨ T_exists T_trail
+      (close 0
+         (psubstitute template
+            (List.combine xs (List.map (fun key : tree => app f (pp key (fvar m term_var))) keys))
+            term_var) m) =
+  T_exists_vars ys T_trail
+    (psubstitute template (List.combine xs (List.map (fun y : nat => app f (fvar y term_var)) ys))
+       term_var)].
+Proof.
+  unfold open_equivalent_types, equivalent_types;
+    repeat step || list_utils || simp_red_top_level_hyp.
+
+  - rewrite substitute_open2 in *; repeat step || list_utils; eauto with wf.
+    rewrite open_close in *; steps; eauto using wfs_combine2 with wf.
+    rewrite (subst_subst template) in *; repeat step || rewrite List.map_map in *.
+    repeat t_substitutions.
+    rewrite list_map_subst in *; steps; eauto.
+    rewrite psubstitute_texists_vars;
+      repeat step || rewrite substitute_trail || rewrite <- satisfies_same_support in *;
+      eauto with fv;
+      eauto using var_in_support.
+    admit.
+Search satisfies.
+    
+
+Require Import Coq.Init.Datatypes.
+Require Import Coq.Lists.List.
+Search (List.map _ (List.map _ _)).
+    admit.
+    admit.
+    apply wf_subst; auto.
+    apply wfs_combine.
+    admit.
+
+  
+  
+intros Γ f template xs ys keys m H.
+
+
+Lemma untangle_open_equivalent_types:
+  forall Γ T1 T2,
+    untangle Γ T1 T2 ->
+    [ Γ ⊨ T1 = T2 ].
+Proof.
+  induction 1; eauto using open_equivalent_types_refl; steps.
+
+
+  
+
+
+  
+Admitted.
+
+(*
+| UntangleFreshen:
+    forall Γ f T T' template xs ys keys m,
+      incomparable (List.map fst keys)
+      (forall k1, k
+      List.NoDup (xs ++ ys) ->
+      T  = substitute template
+        (List.combine xs (List.map (fun key => app f (pp key (fvar m term_var))) keys)) ->
+      T' = substitute template
+        (List.combine xs (List.map (fun y => app f (fvar y term_var)) ys)) ->
+      untangle Γ
+               (T_exists T_trail (close 0 T m))
+               (T_exists_vars ys T_trail T')
+*)
+
+  (*
+| UntangleFreshen:
+    forall Γ T key,
+      untangle Γ
+        (T_exists T_trail (shift_open 1 T (pp key (lvar 0 term_var))))
+        (T_exists T_trail (T_exists T_trail T))
+*)
+  
+
+  (*
+| UntangleFreshen:
+    forall Γ f T T' template xs ys keys m,
+      List.NoDup (xs ++ ys) ->
+      T  = substitute template
+        (List.combine xs (List.map (fun key => app f (pp key (fvar m term_var))) keys)) ->
+      T' = substitute template
+        (List.combine xs (List.map (fun y => app f (fvar y term_var)) ys)) ->
+      untangle Γ
+               (T_exists T_trail (close 0 T m))
+               (T_exists_vars ys T_trail T')
+*)
+
+(*
+
+
+
+(*
+| UntangleTauSingleton:
+    forall Γ f T T' T'' x y z ps,
+(*      List.NoDup (xs ++ ys ++ zs) ->
+      ~ y ∈ fv T'' ->
+      ~ z ∈ fv T'' -> *)
+(*      [ (f: List -> Nat) :: Γ ⊨ f : T_tau ] -> *)
+(*      T = substitute T'' (List.map (fun x => app f (trailOf ps (fvar y term_var))) xs -> *)
+      T  = substitute T'' ((x, app f (trailOf ps (fvar y term_var))) :: nil) ->
+      T' = substitute T'' ((x, app f (fvar z term_var)) :: nil) ->
+      untangle Γ
+               (T_exists List (close 0 T y))
+               (T_exists List (T_exists List (close 1 T' z)))
+*)
+
+
+Fixpoint trailOf (ps: list tree) (t: tree) :=
+  match ps with
+  | nil => t
+  | x :: xs => tcons x (trailOf xs t)
+  end.
+
+Fixpoint trailOf' (ps: list nat) (t: tree) : tree :=
+  match ps with
+  | nil => t
+  | x :: xs => tcons (build_nat x) (trailOf' xs t)
+  end.
+
+Definition append : tree. Admitted.
+Definition apply_append t1 t2 := app (app append t1) t2.
+
+Definition tau_star (f: tree) : Prop :=
+  forall (vs: list nat) (prefixes: list (list nat)),
+    List.NoDup prefixes ->
+    exists suffix, forall v prefix,
+      [ suffix : List ]v ->
+      (v, prefix) ∈ List.combine vs prefixes ->
+      [ app f (trailOf' prefix suffix) ≡ build_nat v ].
+
+Definition tau_star' (f: tree) : Prop :=
+  forall (trails: list tree) (prefixes: list (list nat)),
+    List.NoDup prefixes ->
+    (forall trail, trail ∈ trails -> [ trail : List ]v) ->
+    exists suffix, [ suffix : List ]v /\ forall trail prefix,
+      (trail, prefix) ∈ List.combine trails prefixes ->
+      [ app f (trailOf' prefix suffix) ≡ app f trail ].
+
+Definition T_same_type T1 T2 : tree :=
+  T_intersection
+    (T_forall T1 (T_exists T2 (T_equiv (lvar 0 term_var) (lvar 1 term_var))))
+    (T_forall T2 (T_exists T1 (T_equiv (lvar 0 term_var) (lvar 1 term_var)))).
+
+Definition T_tau': tree :=
+  T_type_refine T_top ( (* f *)
+    T_forall List ( (* prefix *)
+      T_forall List ( (* trail *)
+        T_exists List ( (* suffix *)
+          T_equiv
+            (app (lvar 3 term_var) (lvar 1 term_var))
+            (app (lvar 3 term_var) (apply_append (lvar 2 term_var) (lvar 1 term_var)))
+        )
+      )
+    )
+  ).
+
+
+
+Definition tau_star'' (f: tree) : Prop :=
+  forall (trails: list tree) (prefixes: list (list nat)),
+    List.NoDup prefixes ->
+    (forall trail, trail ∈ trails -> [ trail : List ]v) ->
+    exists suffix, [ suffix : List ]v /\ forall trail prefix,
+      (trail, prefix) ∈ List.combine trails prefixes ->
+      [ app f (trailOf' prefix suffix) ≡ app f trail ].
+
+*)
+
+
+(*
+exists p, { f (1 :: p) } <: exists p, { f p }  OK
+exists p, { f p } <: exists p, { f (1 :: p) }  from Tau
+
+exists p, { (f p, 0) }_Top <: exists p' { (f (1 :: p'), 0) }_Top
+
+let
+  t ≡ (f p, 0) for some p
+  we know there exists p', such that f p ≡ f (1 :: p')
+  t ≡ (f p, 0) ≡ (f (1 :: p'), 0)
+*)
+
+(* WRONG
+exists p p', { (f p, f (1 :: p')) }_Top <: exists p' { (f (1 :: p'), f (1 :: p')) }_Top
+
+let
+  t ≡ (f p, f (1 :: p')) for some p and p'
+
+  we know there exists p'', such that f p ≡ f (1 :: p'')
+  t ≡ (f p, f (1 :: p')) ≡ (f (1 :: p''), (1 :: p'))
+*)
+
+(*
+exists p p', { (f p, g (2 :: p')) }_Top <: exists p' { (f (1 :: p'), g (2 :: p')) }_Top
+
+
+exists p1 p2, { (f nil p1, g nil p2 }_Top <: exists p' { (f [1] p', g [2] p') }_Top
+
+let
+  t ≡ (f p, f (2 :: p')) for some p and p'
+
+  define prefix1 = 1 and prefix2 = 2
+  define trail1 = p, and trail2 = 2 :: p'
+
+by the property, there exists p'' such that
+f (1 :: p'') ≡ f p
+f (2 :: p'') ≡ f (2 :: p')
+
+so t ≡ (f (1 :: p''), f (2 :: p'')) and so
+
+t :  exists p'' { (f (1 :: p''), f (2 :: p'')) }_Top
+
+
+  we know there exists p'', such that f p ≡ f (1 :: p'')
+
+  t ≡ (f p        , f (2 :: p'))
+    ≡ (f (1 :: p''), f (2 :: p'))
+*)
+
+(*
+
+Property for f1, ..., fn:
+
+forall trail1, ..., trailn
+  forall distinct prefix1, ..., prefix_n,
+  exists suffix,
+    f1 (prefix1 ++ suffix)  ≡ f trail1 and
+    ...
+    fn (prefix_n ++ suffix) ≡ f trailn
+*)
+
+(*
+forall v1, ..., vn: Nat
+  forall distinct prefix1, ..., prefix_n,
+  exists suffix,
+    choose (prefix1 ++ suffix)  ≡ v1 and
+    ...
+    choose (prefix_n ++ suffix) ≡ vn
+*)
+
+
+(* def h(p: List)(f: List -> Nat) :=
+     [ ...
+       f [1] p
+*)
+
+(*
+
+[[ t: A ]] = exists x: A, x = t
+
+[[ A <-> B ]] = {{ uu | (A -> B) * (B -> A) }}
+[[ A <-> B ]] = forall x: A, [ x : B ] intersect ...
+
+About choose_nat, we know:
+
+P(choose_nat) =
+  forall v1, ..., vn,
+  forall distinct prefix1, ..., prefix_n,
+  exists suffix,
+    choose_nat (prefix1 ++ suffix) -> v1 and
+    ...
+    choose_nat (prefix_n ++ suffix) -> vn
+
+We want to prove: choose[Nat]: Tau(z, Nat)
+Consider a prefix
+
+( -> ) consider a suffix, and consider choose_nat (prefix ++ suffix) ->* v1
+       for prefix1 = <>
+       there exists suffix1, choose_nat suffix1 ->* v1
+
+( <- ) consider a suffix, and consider choose_nat suffix ->* v1
+       for prefix1 = prefix
+       there exists suffix1, choose_nat (prefix1 ++ suffix1) ->* v1
+
+-------------------------------------------------
+
+The tau property:
+  forall prefix,
+    (exists suffix, { f suffix }) <:
+    (exists suffix, { f (prefix ++ sufix) })
+
+  forall prefix, suffix, exists suffix', f suffix = f (prefix ++ suffix')
+
+  forall prefix, Nat <: exists suffix, { choose (prefix ++ sufix) }
+
+
+tau' property:
+  exists suffix, forall prefix,
+    exists mid, f suffix = f (prefix ++ mid ++ suffix)
+
+
+tau2 property:
+  forall v1, v2
+  forall distinct prefix1, prefix2,
+  exists suffix,
+    choose (prefix1 ++ suffix) -> v1 and
+    choose (prefix2 ++ suffix) -> v2
+
+  forall distinct prefix1, prefix2,
+    Nat * Nat <:
+    exists suffix, { choose (prefix1 ++ sufix), choose (prefix2 ++ suffix)  }
+
+
+taun property:
+  forall v1, ..., vn,
+  forall distinct prefix1, ..., prefix_n,
+  exists suffix,
+    choose_nat (prefix1 ++ suffix) -> v1 and
+    ...
+    choose_nat (prefix_n ++ suffix) -> vn
+
+  forall distinct prefix1, ..., prefix_n,
+    Nat * Nat * ... * Nat <:
+    exists suffix, { choose (prefix1 ++ sufix), ..., choose (prefix_n ++ suffix)  }
+*)
+
+(*
+[ f :
+T_type_refine T_top ( (* f *)
+  T_forall ListListNat ( (* trails *)
+    T_forall ListListNat ( (* prefixes *)
+      T_intersection
+        (no_duplicate prefixes ≡ true)
+        (T_exists ListNat ( (* suffix *)
+          prefixes.map(prefix => app f (apply_append prefix suffix)) ≡
+          trails.map(f)
+*)
+
+(*
+(* forall prefix, trail, exists suffix, f trail = f (prefix ++ suffix) *)
+Definition T_tau: tree :=
+  T_type_refine T_top (
+    T_forall List (T_same_type
+      (T_exists List (T_singleton T_top (app (lvar 2 term_var)
+        (apply_append (lvar 1 term_var) (lvar 0 term_var) ))))
+      (T_exists List (T_singleton T_top (app (lvar 2 term_var) (lvar 0 term_var))))
+    )
+  ).
+*)
